some_iff_isValid

Clap/Lang/FB/FB.lean
@@ -10,32 +10,82 @@ namespace FB
 def true (p : ℕ) [Fact (p ≥ 2)] : FB p := .c 1
 def false (p : ℕ) [Fact (p ≥ 2)] : FB p := .c 0
 
+lemma eval_true {p : ℕ} {varStore : VarStore p} [Fact (p ≥ 2)]:
+  [varStore|true p] = .some 1
+:= by
+  simp [FB.true]
+
+lemma eval_false {p : ℕ} {varStore : VarStore p} [Fact (p ≥ 2)]:
+  [varStore|false p] = .some 0
+:= by
+  simp [FB.false]
+
+@[simp, grind =]
+lemma eval_true_isSome {p : ℕ} {varStore : VarStore p} [Fact (p ≥ 2)]:
+  [varStore|true p].isSome = Bool.true
+:= by
+  grind [eval_true]
+
+@[simp, grind =]
+lemma eval_false_isSome {p : ℕ} {varStore : VarStore p} [Fact (p ≥ 2)]:
+  [varStore|false p].isSome = Bool.true
+:= by
+  grind [eval_false]
+
 variable {p : ℕ} [Fact (p ≥ 2)]
 
 def isValid (x : FB p) (varStore : VarStore p) : Prop :=
   x.eval varStore = .some 0 ∨
   x.eval varStore = .some 1
 
+-- TODO there must be a better way of putting this
+@[grind .]
+lemma isValid_iff_eval_eq_eval_false_or_eval_true
+  {x : FB p} {varStore : VarStore p}
+:
+  x.isValid varStore ↔ (
+    [varStore|x] = [varStore|(false p)] ∨
+    [varStore|x] = [varStore|(true p)]
+  )
+:= by
+  simp [isValid, eval_true, eval_false]
+
 def isAlwaysValid (x : FB p) : Prop :=
   ∀ varStore, x.isValid varStore
 
-def toBool (x : FB p) (varStore : VarStore p) : Bool :=
-  x.eval varStore == .some 1
+def toBool (x : FB p) (varStore : VarStore p) : Option Bool :=
+  [varStore|x].bind (λ x => if x == 1 then Bool.true else if x == 0 then Bool.false else .none)
+
+@[grind =]
+lemma toBool_isSome_eq_true_of_isValid
+  {x : FB p} {varStore : VarStore p}
+  (h_isValid : x.isValid varStore)
+:
+  (x.toBool varStore).isSome = Bool.true
+:= by
+  grind [eval_false, eval_true, toBool]
+
+omit [Fact (p ≥ 2)] in
+@[grind =]
+lemma toBool_isSome_eq_false_of_isValid
+  {x : FB p} {varStore : VarStore p}
+  (h_isValid : ¬x.isValid varStore)
+:
+  (x.toBool varStore).isSome = Bool.false
+:= by
+  simp [isValid] at h_isValid
+  unfold toBool
+  set y := [varStore|x]
+  obtain _ | ⟨y⟩ := y <;> grind
 
 def ofBool (p : ℕ) [Fact (p ≥ 2)] (x : Bool) : FB p :=
-  if x then FB.true p else FB.false p  
+  if x then FB.true p else FB.false p
 
-@[simp, grind .] -- TODO(provisional `simp`)
-lemma eval_ofBool_toBool_of_isValid
-  {p : ℕ}
-  {varStore : VarStore p}
-  (f: FB p)
-  (h : f.isValid varStore)
-  [Fact (p ≥ 2)]
-:
-  (FB.ofBool p (f.toBool varStore)).eval varStore = f.eval varStore
+@[simp, grind =]
+lemma eval_ofBool {p : ℕ} {varStore : VarStore p} [Fact (p ≥ 2)] (b : Bool):
+  [varStore|ofBool p b] = if b then [varStore|true p] else [varStore|false p]
 := by
-  aesop (add simp [toBool,FB.ofBool,FB.isValid])
+  grind [FB.ofBool]
 
 @[simp, grind =]
 lemma toBool_ofBool
@@ -47,6 +97,54 @@ lemma toBool_ofBool
   (FB.ofBool p b).toBool varStore = b
 := by
   aesop (add simp [toBool,FB.ofBool,FB.true,FB.false])
+
+@[simp, grind =]
+lemma toBool_false
+  {varStore : VarStore p}
+:
+  (false p).toBool varStore = Bool.false
+:= by
+  simp [FB.false, FB.toBool]
+
+@[grind =]
+lemma toBool_of_eval_eq_eval_false
+  {varStore : VarStore p}
+  {x : FB p}
+  (h : [varStore|x] = [varStore|false p])
+:
+  x.toBool varStore = .some Bool.false
+:= by
+  grind [FB.toBool, false]
+
+@[grind =]
+lemma toBool_of_eval_eq_eval_true
+  {varStore : VarStore p}
+  {x : FB p}
+  (h : [varStore|x] = [varStore|true p])
+:
+  x.toBool varStore = .some Bool.true
+:= by
+  grind [FB.toBool, true]
+
+@[simp, grind =]
+lemma toBool_true
+  {varStore : VarStore p}
+:
+  (true p).toBool varStore = Bool.true
+:= by
+  simp [FB.true, FB.toBool]
+
+@[simp, grind .] -- TODO(provisional `simp`)
+lemma eval_ofBool_toBool_of_isValid
+  {p : ℕ}
+  {varStore : VarStore p}
+  {x: FB p}
+  (h : x.isValid varStore)
+  [Fact (p ≥ 2)]
+:
+  [varStore|(FB.ofBool p ((x.toBool varStore).get (by grind)))] = [varStore|x]
+:= by
+  grind
 
 namespace ofBool
 
@@ -76,20 +174,20 @@ instance {p} : VarStoreSize p (FB p) where
   toLinear varStore x := #v[x.eval varStore |>.getD 42]
 
 instance : Convert p (FB p) Bool where
-  toIdeal Γ x := .some (FB.toBool x Γ)
+  toIdeal Γ x := FB.toBool x Γ
   toRepresents := FB.ofBool p
-  someOfIsValid := by simp
+  someOfIsValid Γ x := by unfold_projs; grind [IsValid.isValid]
   toIdealtoRepresents := by simp
   toRepresentstoIdeal := by simp
 
 /-
 TODO Provisional simp
 -/
-attribute [simp, grind =] Convert.toIdealtoRepresents Convert.toRepresentstoIdeal 
+attribute [simp, grind =] Convert.toIdealtoRepresents Convert.toRepresentstoIdeal
 
 lemma toIdeal_def {varStore} {x} :
   Convert.toIdeal (representsT := FB p) (idealT := Bool) varStore x =
-  .some (FB.toBool x varStore) := rfl
+  (FB.toBool x varStore) := rfl
 
 lemma toRepresents_def {x} :
   Convert.toRepresents p (representsT := FB p) (idealT := Bool) x =
