Clap/eDSLState/Varstore.lean
@@ -3,6 +3,13 @@ import Std.Data.ExtTreeMap
 
 namespace Clap
 
-abbrev VarStore (p : ℕ) := Std.ExtTreeMap ℕ (ZMod p) (cmp := compare)
+def VarStore (p : ℕ) := Std.ExtTreeMap ℕ (ZMod p) (cmp := compare)
+deriving Inhabited
+
+instance {p : ℕ} : EmptyCollection (VarStore p) := inferInstanceAs (EmptyCollection (Std.ExtTreeMap ℕ (ZMod p)))
+
+instance {p : ℕ} : GetElem? (VarStore p) ℕ (ZMod p) (λ Γ x ↦ Γ.contains x) where
+  getElem  Γ x h := Γ.get x h
+  getElem? Γ x   := Γ.get? x
 
 end Clap
