Clap/Lang/FB/assert.lean
@@ -15,28 +15,61 @@ def matchesUnaryPredicatePure
   (spec_function : Bool → Prop)
   (function : FB p → Edsl.CircuitStateM p Unit)
 : Prop :=
-  ∀ (a : FB p) varStore numAlloc, a.isValid (varStore.get?) →
+  ∀ (a : FB p) varStore numAlloc, a.isValid (varStore) →
     let ⟨numAllocPost, varStorePost, constraints⟩ := Edsl.CircuitState.eval
-      ((function a).getState numAlloc)
+      ((function a).getCircuit numAlloc)
       varStore
       numAlloc
-    constraints = spec_function (a.toBool varStore.get?) ∧
+    constraints = spec_function (a.toBool varStore) ∧
     numAllocPost = numAlloc ∧
     varStorePost = varStore
 
 def spec (p : ℕ) [Fact (p ≥ 2)] : Prop := matchesUnaryPredicatePure p (·) FB.assert
 
+lemma aux
+  {p : ℕ}
+  {varStore : VarStore p}
+  [Fact (p ≥ 2)]
+  {a : FB p}
+:
+  [varStore|a] = [varStore|false p] →
+  [varStore|a.not] = [varStore|FB.ofBool p ((λ x => !x) (FB.toBool (false p) varStore))]
+:= by
+  simp
+  have := FB.not.equiv (p := p)
+  have :=
+
+  intro h_a_false
+  specialize this a varStore (by simp [h_a_false, IsValid.isValid, FB.isValid, eval_false])
+  simp at this
+  have :
+    [varStore|a.not] = [varStore|Convert.toRepresents p (Convert.toIdeal varStore a.not).get (Convert.someOfIsValid)]
+
 lemma equiv (p : ℕ) [Fact (p ≥ 2)] :
   spec p
 := by
   intro a varStore numAlloc h_isValid
-  simp [
-    Clap.monads,
-    FB.assert,
-    h_isValid,
-    not.equiv a,
-    ofBool.equiv
-  ]
+  have := FB.not.equiv (p := p)
+  simp [FB.assert]
+  have :
+    unconstrained[numAlloc][varStore][a.not]? =
+    unconstrained[numAlloc][varStore][FB.ofBool p ((fun x => !x) (a.toBool varStore))]?
+  := by
+    unfold matchesUnaryFunction at this
+    specialize this a varStore h_isValid
+    simp [Convert.toIdeal, FB.toBool] at this
+    simp [getElem?, FB.toBool]
+    apply isValid_iff_eval_eq_eval_false_or_eval_true.mp at h_isValid
+    grind
+    obtain h_val | h_val := h_isValid
+    -- have : [varStore|a.not] = [varStore|a]
+    <;> simp [h_val, this]
+
+  have getElem?_unconstrained (e : FixedExp p):
+    unconstrained[numAlloc][varStore][e]? =
+    [varStore|e]
+  := rfl
+  simp [this, getElem?_unconstrained]
 
 end assert
 
